Transformations/Alpha_Equiv_Bigstep_Correct.thy
@@ -21,6 +21,9 @@ fun alpha_equiv_Result ::
 (* TODO: should we care about the order of locals?
  * should we make sure all variables in l1 and l2 are accounted for? *)
 
+(* NB: this works only because we disallow shadowing.
+ *)
+(*
 fun alpha_equiv_local_variables'l ::
   "(name * name) list \<Rightarrow> (Identifier * Value) list \<Rightarrow> (Identifier * Value) list \<Rightarrow> bool" where
 "alpha_equiv_local_variables'l [] vm1 vm2 = True"
@@ -32,34 +35,388 @@ fun alpha_equiv_local_variables'l ::
      None \<Rightarrow> False
      | Some val2 \<Rightarrow>
       (val1 = val2 \<and> alpha_equiv_local_variables'l nt vm1 vm2)))"
+*)
 
-lift_definition alpha_equiv_local_variables' ::
-  "(name, name) oalist \<Rightarrow> (Identifier * Value) list \<Rightarrow> (Identifier * Value) list \<Rightarrow> bool"
-is alpha_equiv_local_variables'l
-  .
+definition alpha_equiv_local_variables' ::
+  "(name, name) oalist \<Rightarrow> (Identifier * Value) list \<Rightarrow> (Identifier * Value) list \<Rightarrow> bool" where
+"alpha_equiv_local_variables' subst vm1 vm2 =
+  (oalist_all (\<lambda> (n1, n2) .
+    (case map_of vm1 n1 of
+      None \<Rightarrow> False
+      | Some val1 \<Rightarrow>
+        (case map_of vm2 n2 of
+          None \<Rightarrow> False
+          | Some val2 \<Rightarrow> val1 = val2))) subst)"
 
-fun alpha_equiv_local_variables ::
+(* make sure that our oalist substitution captures all the local variables. *)
+
+definition alpha_equiv_local_variables ::
   "subst \<Rightarrow> (Identifier * Value) list \<Rightarrow> (Identifier * Value) list \<Rightarrow> bool" where
-"alpha_equiv_local_variables [] [] [] = True"
-| "alpha_equiv_local_variables (sh#st) (v1h#v1t) (v2h#v2t) =
-   (alpha_equiv_local_variables' sh v1h v2h \<and>
-    \<comment> \<open>oalist_len sh = oalist_len v1h \<and> \<close>
-    oalist_keys sh = oalist_keys v1h \<and>
-    \<comment> \<open> oalist_len sh = oalist_len v2h \<and> \<close>
-    oalist_one_one sh \<and>
-    oalist_keys (oalist_flip sh) = oalist_keys v2h \<and>
-    alpha_equiv_local_variables st v1t v2t)"
-| "alpha_equiv_local_variables _ _ _ = False"
+"alpha_equiv_local_variables subst vm1 vm2 =
+  (list_all (\<lambda> subst' . alpha_equiv_local_variables' subst' vm1 vm2) subst \<and>
+   list_all oalist_one_one subst \<and>
+   list_all (\<lambda> (k, v) . 
+    (case subst_get subst k of
+      Some _ \<Rightarrow> True
+      | _ \<Rightarrow> False)) vm1 \<and>
+   list_all (\<lambda> (k, v) . 
+    (case subst_get (map oalist_flip subst) k of
+      Some _ \<Rightarrow> True
+      | _ \<Rightarrow> False)) vm2)"
 
+(* function equivalence
+*)
+
+type_synonym FunctionContext =
+  \<open>(Identifier\<times> (Statement \<times> Identifier list)) list\<close>
+
+(* TODO: make sure that the way we are making use of the "visible"
+ * identifiers is correct.
+ *)
+definition alpha_equiv_function_contexts' ::
+  "(name, name) oalist \<Rightarrow> FunctionContext \<Rightarrow> FunctionContext \<Rightarrow> bool" where
+"alpha_equiv_function_contexts' subst vm1 vm2 =
+  oalist_all (\<lambda> (n1, n2) .
+    (case map_of vm1 n1 of
+      None \<Rightarrow> False
+      | Some (FunctionDefinition n1' params1 rets1 body1, ids1) \<Rightarrow>
+        (case map_of vm2 n2 of
+          None \<Rightarrow> False
+          | Some (FunctionDefinition n2' params2 rets2 body2, ids2) \<Rightarrow> 
+            (n1 = n1' \<and> n2 = n2' \<and>
+            alpha_equiv_statement [to_oalist (zip ids1 ids2)] [Oalist.empty]
+              (FunctionDefinition n1' params1 rets1 body1)
+              (FunctionDefinition n2' params2 rets2 body2))))) subst"
+
+definition alpha_equiv_function_contexts ::
+  "subst \<Rightarrow> FunctionContext \<Rightarrow> FunctionContext \<Rightarrow> bool" where
+"alpha_equiv_function_contexts subst vm1 vm2 =
+  (list_all (\<lambda> subst' . alpha_equiv_function_contexts' subst' vm1 vm2) subst \<and>
+   list_all (\<lambda> (k, v) . 
+    (case subst_get subst k of
+      Some _ \<Rightarrow> True
+      | _ \<Rightarrow> False)) vm1 \<and>
+   list_all (\<lambda> (k, v) . 
+    (case subst_get (map oalist_flip subst) k of
+      Some _ \<Rightarrow> True
+      | _ \<Rightarrow> False)) vm2)"
 
 (* TODO: ignoring builtins for now *)
 definition alpha_equiv_yulcontext ::
   "subst \<Rightarrow> subst \<Rightarrow> 'g yulcontext \<Rightarrow> 'g yulcontext \<Rightarrow> bool" where
 "alpha_equiv_yulcontext fsubst vsubst c1 c2 =
  (GlobalState c1 = GlobalState c2 \<and>
-  alpha_equiv_Result (Status c1) (Status c2)
-  \<comment> \<open>alpha_equiv_local_variables subst (LocalVariables c1) (LocalVariables c2)\<and>
-      alpha_equiv_functions fvusbst vsubst (Functions c1) (Functions c2)\<close>)"
+  alpha_equiv_Result (Status c1) (Status c2) \<and>
+  alpha_equiv_local_variables vsubst (LocalVariables c1) (LocalVariables c2)\<and>
+  alpha_equiv_function_contexts fsubst (Functions c1) (Functions c2))"
+
+(* result of running the state monad *)
+type_synonym ('g, 'a) yulout = "('a * 'g yulcontext)"
+
+(* for unpacking the State constructor *)
+type_synonym ('g, 'a) yulstatef = "'g yulcontext \<Rightarrow> ('a * 'g yulcontext)"
+
+lemma alpha_equiv_getLocalVariable :
+  assumes "alpha_equiv_local_variables vsubst lv1 lv2"
+  assumes "LocalVariables c1 = lv1"
+  assumes "LocalVariables c2 = lv2"
+  assumes "alpha_equiv_name vsubst id1 id2"
+  shows "getLocalVariable c1 id1 = getLocalVariable c2 id2"
+  using assms
+  sorry
+(*
+proof(induction lv1 arbitrary: vsubst lv2 c1 c2 id1 id2)
+  case Nil1 : Nil
+  then show ?case
+    apply(auto simp add: alpha_equiv_local_variables_def)
+next
+  case (Cons substh substt)
+  show ?case
+  proof(cases "get substh id1")
+    case None1 : None
+
+    show ?thesis
+    proof(cases "get (oalist_flip substh) id2")
+      case None2 : None
+      then show ?thesis
+        using Cons None1
+        apply(auto simp add: alpha_equiv_local_variables_def)
+    next
+      case (Some a)
+      then show ?thesis sorry
+    qed
+
+    then show ?thesis
+      using Cons
+      apply(auto simp add: alpha_equiv_local_variables_def)
+    then show ?thesis sorry
+  next
+    case Some1 : (Some id1')
+
+    show ?thesis
+      using Cons
+      apply(auto simp add: alpha_equiv_local_variables_def)
+
+    then show ?thesis sorry
+  qed
+
+  then show ?case
+    apply(auto simp add: alpha_equiv_local_variables_def)
+qed
+*)
+
+(* State_Monad.state.rel_state :: "('a \<Rightarrow> 'b \<Rightarrow> bool) \<Rightarrow> ('c, 'a) state \<Rightarrow> ('c, 'b) state \<Rightarrow> bool" *)
+(* run_state :: "('s, 'a) state \<Rightarrow> 's \<Rightarrow> 'a \<times> 's" *)
+
+lemma alpha_equiv_correct :
+  shows "(\<forall> fsubst vsubst (c1 :: 'g yulcontext) (c2 :: 'g yulcontext).
+  ((\<forall> st1 st2 m m1 m2 c1' c2'. 
+    alpha_equiv_statement fsubst vsubst st1 st2 \<longrightarrow>
+    alpha_equiv_yulcontext fsubst vsubst c1 c2 \<longrightarrow>
+    run_state (evalStatement n m st1) c1 = (m1, c1') \<longrightarrow>
+    run_state (evalStatement n m st2) c2 = (m2, c2') \<longrightarrow>
+    (alpha_equiv_yulcontext fsubst vsubst c1' c2' \<and> m1 = m2)) \<and>
+   (\<forall> e1 e2 c1' c2' vals1 vals2.
+    alpha_equiv_expr fsubst vsubst e1 e2 \<longrightarrow>
+    alpha_equiv_yulcontext fsubst vsubst c1 c2 \<longrightarrow>
+    run_state (evalExpression n e1) c1 = (vals1, c1') \<longrightarrow>
+    run_state (evalExpression n e2) c2 = (vals2, c2') \<longrightarrow>
+    (alpha_equiv_yulcontext fsubst vsubst c1' c2' \<and> vals1 = vals2)) \<and>
+   (\<forall> e1 e2 c1' c2' v1 v2.
+    alpha_equiv_expr fsubst vsubst e1 e2 \<longrightarrow>
+    alpha_equiv_yulcontext fsubst vsubst c1 c2 \<longrightarrow>
+    run_state (evalUnaryExpression n e1) c1 = (v1, c1') \<longrightarrow>
+    run_state (evalUnaryExpression n e2) c2 = (v2, c2') \<longrightarrow>
+    (alpha_equiv_yulcontext fsubst vsubst c1' c2' \<and> v1 = v2))))"
+proof(induction n)
+  case 0
+  then show ?case 
+(* TODO: make this nicer and not rely on case_tac *)
+    by(auto simp add: run_state_def errorState_def alpha_equiv_yulcontext_def;
+        case_tac m; auto simp add: errorState_def State_Monad.return_def)
+next
+  case (Suc n)
+
+  have IH1 :
+    "\<And> fsubst vsubst (c1 :: 'g yulcontext) (c2 :: 'g yulcontext) st1 st2 m m1 m2 c1' c2'.
+         alpha_equiv_statement fsubst vsubst
+          st1 st2 \<Longrightarrow>
+         alpha_equiv_yulcontext fsubst vsubst
+          c1 c2 \<Longrightarrow>
+         run_state (evalStatement n m st1) c1 =
+         (m1, c1') \<Longrightarrow>
+         run_state (evalStatement n m st2) c2 =
+         (m2, c2') \<Longrightarrow>
+         alpha_equiv_yulcontext fsubst vsubst
+          c1' c2' \<and>
+         m1 = m2"
+    using Suc.IH
+    by fast
+
+  have IH2 :
+    "\<And> fsubst vsubst (c1 :: 'g yulcontext) (c2 :: 'g yulcontext) e1 e2 c1' c2' vals1 vals2.
+      alpha_equiv_expr fsubst vsubst e1 e2 \<Longrightarrow>
+      alpha_equiv_yulcontext fsubst vsubst c1 c2 \<Longrightarrow>
+      run_state (evalExpression n e1) c1 = (vals1, c1') \<Longrightarrow>
+      run_state (evalExpression n e2) c2 = (vals2, c2') \<Longrightarrow>
+      alpha_equiv_yulcontext fsubst vsubst c1' c2' \<and> vals1 = vals2"
+    using Suc.IH
+    by fast
+
+  have IH3 :
+    "\<And> fsubst vsubst (c1 :: 'g yulcontext) (c2 :: 'g yulcontext) e1 e2 c1' c2' v1 v2.
+    alpha_equiv_expr fsubst vsubst e1 e2 \<Longrightarrow>
+    alpha_equiv_yulcontext fsubst vsubst c1 c2 \<Longrightarrow>
+    run_state (evalUnaryExpression n e1) c1 = (v1, c1') \<Longrightarrow>
+    run_state (evalUnaryExpression n e2) c2 = (v2, c2') \<Longrightarrow>
+    alpha_equiv_yulcontext fsubst vsubst c1' c2' \<and> v1 = v2"
+    using Suc.IH
+    by fast
+
+  have Conc1 : 
+    "\<And> fsubst vsubst (c1 :: 'g yulcontext) (c2 :: 'g yulcontext)
+        st1 st2 m m1 m2 c1' c2'.
+          alpha_equiv_statement fsubst vsubst st1 st2 \<Longrightarrow>
+          alpha_equiv_yulcontext fsubst vsubst c1 c2 \<Longrightarrow>
+          run_state (evalStatement (Suc n) m st1) c1 = (m1, c1') \<Longrightarrow>
+          run_state (evalStatement (Suc n) m st2) c2 = (m2, c2') \<Longrightarrow>
+          alpha_equiv_yulcontext fsubst vsubst c1' c2' \<and>
+          m1 = m2"
+  proof-
+    fix fsubst vsubst
+    fix c1 c2 :: "'g yulcontext"
+    fix st1 st2 m m1 m2 c1' c2'
+
+    assume Hstatement : "alpha_equiv_statement fsubst vsubst st1 st2"
+    assume Hctx : "alpha_equiv_yulcontext fsubst vsubst c1 c2"
+    assume Hrun1 : "run_state (evalStatement (Suc n) m st1) c1 = (m1, c1')"
+    assume Hrun2 : "run_state (evalStatement (Suc n) m st2) c2 = (m2, c2')"
+
+    show "alpha_equiv_yulcontext fsubst vsubst c1' c2' \<and>
+       m1 = m2"
+      sorry
+  qed
+
+  have Conc2 : 
+    "\<And> fsubst vsubst (c1 :: 'g yulcontext) (c2 :: 'g yulcontext)
+      e1 e2 c1' c2' vals1 vals2.
+        alpha_equiv_expr fsubst vsubst e1 e2 \<Longrightarrow>
+        alpha_equiv_yulcontext fsubst vsubst c1 c2 \<Longrightarrow>
+        run_state (evalExpression (Suc n) e1) c1 = (vals1, c1') \<Longrightarrow>
+        run_state (evalExpression (Suc n) e2) c2 = (vals2, c2') \<Longrightarrow>
+        alpha_equiv_yulcontext fsubst vsubst c1' c2' \<and>
+        vals1 = vals2"
+  proof-
+    fix fsubst vsubst
+    fix c1 c2 :: "'g yulcontext"
+    fix e1 e2 c1' c2' vals1 vals2
+
+    assume Hexpr : "alpha_equiv_expr fsubst vsubst e1 e2" 
+    assume Hctx : "alpha_equiv_yulcontext fsubst vsubst c1 c2"
+    assume Hrun1 : "run_state (evalExpression (Suc n) e1) c1 = (vals1, c1')"
+    assume Hrun2 : "run_state (evalExpression (Suc n) e2) c2 = (vals2, c2')"
+
+    show "alpha_equiv_yulcontext fsubst vsubst c1' c2' \<and>
+       vals1 = vals2"
+    proof(cases e1)
+      case Fc1 : (FunctionCall x11 x12)
+      then show ?thesis sorry
+    next
+      case Id1 : (Identifier i1)
+
+      then obtain i2 where Id2 : "e2 = Identifier i2"
+        using Hexpr
+        by(cases e2; auto)
+
+      show ?thesis
+      proof(cases "getLocalVariable c1 i1")
+        case None1 : None
+
+(* need lemma relating getLocalVariable to alpha_equiv_local_variables *)
+        then have None2 : "getLocalVariable c2 i2 = None"
+          using Hexpr Hrun1 Hrun2 Id1 Id2 Hctx
+          apply(cases "getLocalVariable c2 i2"; auto simp add: errorState_def alpha_equiv_yulcontext_def ValueOfIdentifier_def)
+        then show ?thesis
+          using Hexpr Hrun1 Hrun2 Id1 Id2
+          apply(auto simp add: errorState_def alpha_equiv_yulcontext_def ValueOfIdentifier_def)
+
+      next
+        case (Some a)
+        then show ?thesis sorry
+      qed
+
+(* get_local_variable *)
+      then show ?thesis using Hexpr Hctx Hrun1 Hrun2 Id1
+        apply(auto simp add: ValueOfIdentifier_def)
+
+
+      then show ?thesis sorry
+    next
+      case L1 : (Literal v1)
+
+      then obtain v2 where L2 : "e2 = Literal v2"
+        using Hexpr
+        by(cases e2; auto)
+
+      then show ?thesis using Hexpr Hctx Hrun1 Hrun2 L1
+        by(auto)
+    qed
+  qed
+
+  have Conc3 :
+    "\<And> fsubst vsubst (c1 :: 'g yulcontext) (c2 :: 'g yulcontext) e1 e2 c1' c2' v1 v2.
+          alpha_equiv_expr fsubst vsubst e1 e2 \<Longrightarrow>
+          alpha_equiv_yulcontext fsubst vsubst c1 c2 \<Longrightarrow>
+          run_state (evalUnaryExpression (Suc n) e1) c1 = (v1, c1') \<Longrightarrow>
+          run_state (evalUnaryExpression (Suc n) e2) c2 = (v2, c2') \<Longrightarrow>
+          alpha_equiv_yulcontext fsubst vsubst c1' c2' \<and>
+          v1 = v2"
+  proof-
+    fix fsubst vsubst
+    fix c1 c2 :: "'g yulcontext"
+    fix e1 e2 c1' c2' v1 v2
+
+    assume Hexpr : "alpha_equiv_expr fsubst vsubst e1 e2" 
+    assume Hctx : "alpha_equiv_yulcontext fsubst vsubst c1 c2"
+    assume Hrun1 : "run_state (evalUnaryExpression (Suc n) e1) c1 = (v1, c1')"
+    assume Hrun2 : "run_state (evalUnaryExpression (Suc n) e2) c2 = (v2, c2')"
+
+    obtain rest1 :: "('g, Value list) yulstatef" where Rest1 :
+      "evalExpression n e1 = State rest1"
+      by(cases "evalExpression n e1 :: ('g, Value list) yulstate"; auto)
+
+    obtain rest2 :: "('g, Value list) yulstatef" where Rest2 :
+      "evalExpression n e2 = State rest2"
+      by(cases "evalExpression n e2 :: ('g, Value list) yulstate"; auto)
+
+    obtain v1a c1a where Run1a : "run_state (evalExpression n e1) c1 = (v1a, c1a)"
+      by force
+
+    obtain v2a c2a where Run2a : "run_state (evalExpression n e2) c2 = (v2a, c2a)"
+      by force
+
+    have IndHyp : "alpha_equiv_yulcontext fsubst vsubst c1a c2a" "v1a = v2a"
+      using IH2[OF Hexpr Hctx Run1a Run2a] 
+      by auto
+
+    show "alpha_equiv_yulcontext fsubst vsubst c1' c2' \<and>
+       v1 = v2"
+    proof(cases v1a)
+      case V1a_Nil : Nil
+
+      have V2a_Nil : "v2a = []"
+        using Hexpr Hctx Hrun1 Hrun2 Run1a Run2a V1a_Nil
+        using IndHyp
+        by(cases v2a; auto)
+
+      then show ?thesis
+        using Hexpr Hctx Hrun1 Hrun2 Run1a Run2a V1a_Nil 
+        using IndHyp
+        by(auto simp add: errorState_def alpha_equiv_yulcontext_def)
+    next
+      case V1a_Cons1 : (Cons v1ah v1at)
+
+      obtain v2ah v2at where V2a_Cons1 : "v2a = v2ah # v2at"
+        using Hexpr Hctx Hrun1 Hrun2 Run1a Run2a V1a_Cons1 
+        using IndHyp
+        by(cases v2a; auto)
+
+      show ?thesis
+      proof(cases v1at)
+        case V1at_Nil : Nil
+
+        have V2at_Nil : "v2at = []"
+          using Hexpr Hctx Hrun1 Hrun2 Run1a Run2a V1at_Nil V1a_Cons1 V2a_Cons1
+          using IndHyp
+          by(cases v2at; auto)
   
+        then show ?thesis
+          using Hexpr Hctx Hrun1 Hrun2 Run1a Run2a V1a_Cons1 V2a_Cons1 
+          using IndHyp
+          by(auto simp add: errorState_def alpha_equiv_yulcontext_def)
+
+      next
+        case V1a_Cons2 : (Cons v1ah' v1at')
+
+        obtain v2ah' v2at' where V2a_Cons2 : "v2at = v2ah' # v2at'"
+          using Hexpr Hctx Hrun1 Hrun2 Run1a Run2a V1a_Cons1 V2a_Cons1 V1a_Cons2
+          using IndHyp
+          by(cases v2at; auto)
+
+        then show ?thesis
+          using Hexpr Hctx Hrun1 Hrun2 Run1a Run2a V1a_Cons1 V2a_Cons1 V1a_Cons2
+          using IndHyp
+          by(auto simp add: errorState_def alpha_equiv_yulcontext_def)
+      qed
+    qed
+  qed
+
+  show ?case sorry
+(*
+    using Conc1 Conc2 Conc3
+    by fast
+*)
+qed
+
 
 end
